x86/MCSep.v
@@ -63,12 +63,304 @@ Proof.
   - auto.
 Defined.
 
-Axiom transf_prog_combine : 
+
+Lemma transl_instr_from_flat_asm_succeeds:
+  forall o i s0 i1 l i1',
+    is_valid_label l i1' ->
+    FlatAsmgen.transl_instr o i s0 i1 = OK i1' ->
+    exists ins, transl_instr l i i1' = OK ins.
+Proof.
+  unfold FlatAsmgen.transl_instr.
+  intros o i s0 i1 l i1' H0 H1.
+  repeat destr_in H1; simpl in *; eauto.
+  - unfold get_lbl_offset. destr. simpl. eauto.
+  - unfold get_lbl_offset. destr. simpl. eauto.
+  - unfold get_lbl_offset. destr. simpl. eauto.
+  - assert (forall s, exists o, get_lbl_list_offset l i tbl s = OK o).
+    {
+      revert H0. induction 1; simpl; intros; eauto.
+      unfold get_lbl_offset. destr. simpl. edestruct IHForall as (oo & EQ); eauto.
+      rewrite EQ. simpl; eauto.
+    }
+    edestruct H as (oo & EQ). erewrite EQ. simpl. eauto.
+Qed.
+
+Lemma transl_instrs_from_flat_asm_succeeds:
+  forall i s0 c i0 x0 x1 l,
+    Forall (is_valid_label l) x1 ->
+    FlatAsmgen.transl_instrs i s0 i0 c = OK (x0, x1) ->
+    exists ins, transl_instrs l i x1 = OK ins.
+Proof.
+  induction c; simpl; intros; eauto.
+  inv H0; simpl; eauto.
+  monadInv H0.
+  simpl. inv H.
+  edestruct transl_instr_from_flat_asm_succeeds as (ins & TI); eauto.
+  rewrite TI. simpl.
+  edestruct IHc as (inss & TIS); eauto.
+  rewrite TIS. simpl; eauto.
+Qed.
+
+Lemma transl_globdef_from_flat_asm_succeeds:
+  forall g l i d1 d2,
+    (forall f, snd (fst d2) = Some (Gfun (Internal f)) -> Forall (is_valid_label l) (fn_code f)) ->
+    FlatAsmgen.transl_globdef g i d1 = OK d2 ->
+    exists d3, transl_globdef l d2 = OK d3.
+Proof.
+  unfold FlatAsmgen.transl_globdef, transl_globdef.
+  intros g l i d1 d2 VL TG.
+  repeat destr_in TG; eauto.
+  monadInv H0.
+  unfold FlatAsmgen.transl_fun in EQ. repeat destr_in EQ.
+  monadInv H0. repeat destr_in EQ0. simpl. unfold transl_fun. simpl.
+  edestruct transl_instrs_from_flat_asm_succeeds as (inss & TIS).
+  simpl in VL. apply VL. eauto. eauto. simpl in TIS.
+  rewrite TIS. simpl. eauto.
+Qed.
+
+Lemma
+  transl_globdefs_from_flat_asm_succeeds:
+  forall g l d1 d2,
+    Forall (fun '(_,d,_) => forall f, d = Some (Gfun (Internal f)) -> Forall (is_valid_label l) (fn_code f)) d2 ->
+    FlatAsmgen.transl_globdefs g d1 = OK d2 ->
+    exists d3, transl_globdefs l d2 = OK d3.
+Proof.
+  induction d1; simpl; intros; eauto.
+  inv H0; simpl; eauto.
+  destr_in H0. monadInv H0. simpl.
+  edestruct transl_globdef_from_flat_asm_succeeds as (oo & EQQ); eauto.
+  inv H. repeat destr_in H2. simpl; intros; subst. simpl. eauto.
+  inv H.
+  edestruct IHd1 as (ins & TG); eauto. rewrite TG. rewrite EQQ. simpl; eauto.
+Qed.
+
+Lemma transl_globdefs_back:
+  forall defs g tdefs x,
+    FlatAsmgen.transl_globdefs g defs = OK tdefs ->
+    In x tdefs ->
+    exists i y, In (i,y) defs /\ FlatAsmgen.transl_globdef g i y = OK x.
+Proof.
+  induction defs; simpl; intros; eauto. inv H; easy.
+  destr_in H. monadInv H. simpl in H0. destruct H0.
+  - subst. do 2 eexists; split. left; eauto. auto.
+  - edestruct IHdefs as (ii & y & IN & TG); eauto.
+Qed.
+
+Lemma update_maps_labels:
+  forall defs g l c d g' l' c' d',
+    list_norepet (map fst defs) ->
+    (forall i, In i (map fst defs) -> forall lab, l i lab = None) ->
+    FlatAsmgen.update_maps g l c d defs = (g',l',c',d') ->
+    forall i lab,
+      l' i lab <> None <-> (l i lab <> None \/ exists f, In (i,Some (Gfun (Internal f))) defs /\ In lab (FlatAsmgen.labels (Asm.fn_code f))).
+Proof.
+  induction defs; simpl; intros g l c d g' l' c' d' LNR NOLAB UM i lab.
+  - inv UM. split. tauto. intros [A|(? & [] & ?)]; auto.
+  - destruct a. rewrite FlatAsmgenproof.update_maps_cons in UM. repeat destr_in UM. 
+    erewrite IHdefs. 4: eauto.
+    split.
+    + intros [A | (f & IN1 & IN2)]; eauto.
+      * erewrite FlatAsmgenproof.update_lmap in A. 2: eauto.
+        repeat destr_in A. subst.
+        right. eexists; split. left. eauto.
+        simpl in LNR. inv LNR.
+        simpl in *. destr_in Heqp.
+        simpl in *.
+        inv Heqp.
+        destruct (in_dec peq lab (FlatAsmgen.labels (Asm.fn_code f0))). auto.
+        eapply FlatAsmgenproof.update_instrs_other_label in Heqp0; eauto.
+        rewrite Heqp0 in A. destruct A. apply NOLAB. auto.
+    + intros [A | (f & IN1 & IN2)]; eauto.
+      * erewrite FlatAsmgenproof.update_lmap. 2: eauto.
+        repeat destr. subst.
+        simpl in *. destr_in Heqp.
+        simpl in *.
+        inv Heqp.
+        rewrite NOLAB in A. congruence. auto.
+      * destruct IN1 as [A|IN1]; eauto. inv A.
+        simpl in *. repeat destr_in Heqp.
+        edestruct FlatAsmgenproof.update_instrs_in_lbl as (sid & ofs & EQ); eauto.
+        rewrite EQ. left; congruence.
+    + inv LNR; auto.
+    + intros. erewrite FlatAsmgenproof.update_lmap. 2: eauto.
+      simpl in LNR. inv LNR.
+      erewrite <- (NOLAB i1) with (lab := lab0); auto.
+      repeat destr. 
+Qed.
+
+
+Lemma make_maps_labels:
+  forall p g l c d,
+    list_norepet (map fst (AST.prog_defs p)) ->
+    FlatAsmgen.make_maps p = (g,l,c,d) ->
+    forall i lab,
+      l i lab <> None <-> exists f, In (i,Some (Gfun (Internal f))) (AST.prog_defs p) /\ In lab (FlatAsmgen.labels (Asm.fn_code f)).
+Proof.
+  unfold FlatAsmgen.make_maps. intros.
+  erewrite update_maps_labels. 4: eauto.
+  unfold FlatAsmgen.default_label_map. intuition tauto.
+  auto.
+  unfold FlatAsmgen.default_label_map. auto.
+Qed.
+
+Lemma transl_instrs_valid_label:
+  forall labs i l c s0 i0 x x0,
+    Forall
+      (fun i1 : Asm.instruction =>
+         forall lab : label, FlatAsmgen.has_label i1 lab -> In lab labs) c ->
+    (forall lab : label, In lab labs -> l i lab <> None) ->
+    (* list_norepet (FlatAsmgen.labels c) -> *)
+    FlatAsmgen.transl_instrs i s0 i0 c = OK (x, x0) ->
+    Forall (is_valid_label l) x0.
+Proof.
+  induction c; simpl; intros s0 i0 x x0 H H0 H1; eauto.
+  inv H1. constructor.
+  monadInv H1.
+  inv H.
+  constructor; eauto.
+  - destruct a; simpl in EQ; inv EQ; simpl in *; auto.
+    rewrite Forall_forall; intros; apply H0. auto.
+Qed.
+
+Lemma transl_fun_valid_label:
+  forall g i f tf l,
+    FlatAsmgen.transl_fun g i f = OK tf ->
+    Forall (fun i => forall lab, FlatAsmgen.has_label i lab -> In lab (FlatAsmgen.labels (Asm.fn_code f)))
+           (Asm.fn_code f) ->
+    (forall lab,
+        In lab (FlatAsmgen.labels (Asm.fn_code f)) ->
+        l i lab <> None) ->
+    Forall (is_valid_label l) (fn_code tf).
+Proof.
+  intros g i f tf l TF FC LS.
+  unfold FlatAsmgen.transl_fun in TF.
+  repeat destr_in TF. monadInv H0.
+  repeat destr_in EQ0. simpl.
+  eapply transl_instrs_valid_label. 3: eauto.
+  eauto. auto.
+Qed.
+
+Lemma transf_prog_combine : 
   forall (p1 p2: FlatAsm.program) (tp1 tp2: MC.program) p
     (LK: link p1 p2 = Some p)
     (TF1: transf_program p1 = OK tp1)
     (TF2: transf_program p2 = OK tp2),
   exists tp, transf_program p = OK tp.
+Proof.
+  simpl.
+  unfold link_flatasmprog.
+  intros p1 p2 tp1 tp2 p LK TF1 TF2.
+  repeat destr_in LK.
+  unfold transf_program in *.
+  repeat destr_in TF1. repeat destr_in TF2.
+  monadInv H0. monadInv H1.
+  unfold FlatAsmgen.transf_program in Heqr.
+  repeat destr_in Heqr.
+  rewrite pred_dec_true.
+  rewrite pred_dec_true.
+  replace (check_faprog p) with (true).
+  unfold FlatAsmgen.transl_prog_with_map in H0.
+  monadInv H0. simpl.
+  cut (exists l', transl_globdefs l x1 = OK l').
+  intros (l' & TG). rewrite TG; simpl; eauto.
+  eapply transl_globdefs_from_flat_asm_succeeds.
+  {
+    rewrite Forall_forall. intros x2 IN.
+    eapply transl_globdefs_back in IN. 2: eauto. simpl in IN.
+    destruct IN as (i & y & IN & TG).
+    repeat destr. intros; subst.
+    inv w.
+    pose proof (make_maps_labels _ _ _ _ _ wf_prog_norepet_defs Heqp3) as LABSPEC.
+    unfold FlatAsmgen.transl_globdef in TG. repeat destr_in TG.
+    monadInv H0.
+    red in wf_prog_valid_labels.
+    rewrite Forall_forall in wf_prog_valid_labels.
+    specialize (wf_prog_valid_labels _ IN).
+    simpl in wf_prog_valid_labels.
+    red in wf_prog_valid_labels.
+    eapply transl_fun_valid_label; eauto.
+    intros. rewrite LABSPEC. eexists; split; eauto.
+  }
+  eauto.
+  {
+    unfold FlatAsmgen.transl_prog_with_map in H0. monadInv H0.
+    unfold check_faprog. simpl. symmetry.
+    apply forallb_forall.
+    unfold check_fadef.
+    intros. repeat destr. rewrite andb_true_iff. split.
+    - rewrite forallb_forall. intros. repeat destr.
+    make_maps_labels
+    simpl.
+  unfold code_segid, data_segid. congruence.
+  unfold FlatAsmgen.transl_prog_with_map in H0. monadInv H0. simpl.
+  auto.
+
+
+
+    unfold flatasm_to_asm in Heqo.
+    Transparent Linker_prog. simpl in Heqo.
+    unfold link_prog in Heqo. simpl in Heqo. repeat destr_in Heqo.
+    simpl in *.
+    rewrite Forall_forall. intros x2 IN.
+    eapply transl_globdefs_back in IN. 2: eauto. simpl in IN.
+    destruct IN as (i & y & IN & TG).
+    apply PTree.elements_complete in IN.
+    rewrite PTree.gcombine in IN by auto.
+
+    
+    Lemma link_prog_merge_inv:
+      forall x y z,
+        link_prog_merge (F:=Asm.fundef) (V:= unit) x y = Some z ->
+        x = Some z \/ y = Some z.
+    Proof.
+      destruct x,y; eauto.
+      intros. simpl in H.
+      destruct o, o0; simpl in *; inv H; auto.
+      repeat destr_in H1.
+      Transparent Linker_def. simpl in *. unfold link_def in Heqo.
+      repeat destr_in Heqo; auto.
+      Transparent Linker_fundef.
+      simpl in *.
+      unfold link_fundef in Heqo0.
+      repeat destr_in Heqo0.
+      Transparent Linker_vardef.
+      simpl in *.
+      unfold link_vardef in Heqo0.
+      repeat destr_in Heqo0.
+      Transparent Linker_varinit Linker_unit.
+      simpl in *. inv Heqo. unfold link_varinit in Heqo1.
+      destruct v, v0. simpl in *. apply andb_true_iff in Heqb.
+      destruct Heqb as (Ha & Hb).
+      apply eqb_prop in Ha.
+      apply eqb_prop in Hb. subst.
+      destruct gvar_info, gvar_info0. simpl in *.
+      repeat destr_in Heqo1; eauto.
+    Qed.
+    apply link_prog_merge_inv in IN.
+    repeat destr. intros; subst. simpl in *.
+    unfold link_prog_merge in IN.
+
+    
+
+
+    Transparent Linker_option. simpl in IN.
+    unfold link_option in IN.
+    repeat destr_in IN.
+    Transparent Linker_def. simpl in Heqo3.
+    unfold link_def in Heqo3.
+    unfold link in Heqo3.
+
+
+
+    assert (exists y, (In y x  ))
+  }
+  eauto.
+  admit.
+  unfold FlatAsmgen.transl_prog_with_map in H0. monadInv H0. simpl.
+  unfold code_segid, data_segid. congruence.
+  unfold FlatAsmgen.transl_prog_with_map in H0. monadInv H0. simpl.
+  auto.
+Qed.
 
 Lemma transl_instr_inv : forall l fid i i',
     transl_instr l fid i = OK i' ->
